blocking semantic

examples/hoare_logic/blocking_semantics4/blocking_semantics4_WP_wp_reduction_1.v
@@ -129,6 +129,8 @@ Definition ident_index(v:ident): Z := match v with
   | (mk_ident x) => x
   end.
 
+Parameter result: ident.
+
 Axiom ident_decide : forall (m1:ident) (m2:ident), (m1 = m2) \/ ~ (m1 = m2).
 
 (* Why3 assumption *)
@@ -161,17 +163,19 @@ Axiom fmla_WhyType : WhyType fmla.
 Existing Instance fmla_WhyType.
 
 (* Why3 assumption *)
-Inductive stmt  :=
-  | Sskip : stmt 
-  | Sassign : mident -> term -> stmt 
-  | Sseq : stmt -> stmt -> stmt 
-  | Sif : term -> stmt -> stmt -> stmt 
-  | Sassert : fmla -> stmt 
-  | Swhile : term -> fmla -> stmt -> stmt .
-Axiom stmt_WhyType : WhyType stmt.
-Existing Instance stmt_WhyType.
-
-Axiom decide_is_skip : forall (s:stmt), (s = Sskip) \/ ~ (s = Sskip).
+Inductive expr  :=
+  | Evalue : value -> expr 
+  | Ebin : expr -> operator -> expr -> expr 
+  | Evar : ident -> expr 
+  | Ederef : mident -> expr 
+  | Eassign : mident -> expr -> expr 
+  | Eseq : expr -> expr -> expr 
+  | Elet : ident -> expr -> expr -> expr 
+  | Eif : expr -> expr -> expr -> expr 
+  | Eassert : fmla -> expr 
+  | Ewhile : expr -> fmla -> expr -> expr .
+Axiom expr_WhyType : WhyType expr.
+Existing Instance expr_WhyType.
 
 (* Why3 assumption *)
 Definition type_value(v:value): datatype :=
@@ -252,28 +256,46 @@ Inductive type_fmla : (map mident datatype) -> (list (ident* datatype)%type)
       pi) f) -> (type_fmla sigma pi (Fforall x TYunit f)).
 
 (* Why3 assumption *)
-Inductive type_stmt : (map mident datatype) -> (list (ident* datatype)%type)
-  -> stmt -> Prop :=
-  | Type_skip : forall (sigma:(map mident datatype)) (pi:(list (ident*
-      datatype)%type)), (type_stmt sigma pi Sskip)
+Inductive type_expr : (map mident datatype) -> (list (ident* datatype)%type)
+  -> expr -> datatype -> Prop :=
+  | Type_Evalue : forall (sigma:(map mident datatype)) (pi:(list (ident*
+      datatype)%type)) (v:value), (type_expr sigma pi (Evalue v)
+      (type_value v))
+  | Type_Evar : forall (sigma:(map mident datatype)) (pi:(list (ident*
+      datatype)%type)) (v:ident) (ty:datatype), ((get_vartype v pi) = ty) ->
+      (type_expr sigma pi (Evar v) ty)
+  | Type_Ederef : forall (sigma:(map mident datatype)) (pi:(list (ident*
+      datatype)%type)) (v:mident) (ty:datatype), ((get sigma v) = ty) ->
+      (type_expr sigma pi (Ederef v) ty)
+  | Type_Ebinop : forall (sigma:(map mident datatype)) (pi:(list (ident*
+      datatype)%type)) (e1:expr) (e2:expr) (op:operator) (ty1:datatype)
+      (ty2:datatype) (ty:datatype), (type_expr sigma pi e1 ty1) ->
+      ((type_expr sigma pi e2 ty2) -> ((type_operator op ty1 ty2 ty) ->
+      (type_expr sigma pi (Ebin e1 op e2) ty)))
   | Type_seq : forall (sigma:(map mident datatype)) (pi:(list (ident*
-      datatype)%type)) (s1:stmt) (s2:stmt), (type_stmt sigma pi s1) ->
-      ((type_stmt sigma pi s2) -> (type_stmt sigma pi (Sseq s1 s2)))
+      datatype)%type)) (e1:expr) (e2:expr) (ty:datatype), (type_expr sigma pi
+      e1 TYunit) -> ((type_expr sigma pi e2 ty) -> (type_expr sigma pi
+      (Eseq e1 e2) ty))
   | Type_assigns : forall (sigma:(map mident datatype)) (pi:(list (ident*
-      datatype)%type)) (x:mident) (t:term) (ty:datatype), ((get sigma
-      x) = ty) -> ((type_term sigma pi t ty) -> (type_stmt sigma pi
-      (Sassign x t)))
+      datatype)%type)) (x:mident) (e:expr) (ty:datatype), ((get sigma
+      x) = ty) -> ((type_expr sigma pi e ty) -> (type_expr sigma pi
+      (Eassign x e) TYunit))
   | Type_if : forall (sigma:(map mident datatype)) (pi:(list (ident*
-      datatype)%type)) (t:term) (s1:stmt) (s2:stmt), (type_term sigma pi t
-      TYbool) -> ((type_stmt sigma pi s1) -> ((type_stmt sigma pi s2) ->
-      (type_stmt sigma pi (Sif t s1 s2))))
+      datatype)%type)) (t:expr) (e1:expr) (e2:expr) (ty:datatype),
+      (type_expr sigma pi t TYbool) -> ((type_expr sigma pi e1 ty) ->
+      ((type_expr sigma pi e2 ty) -> (type_expr sigma pi (Eif t e1 e2) ty)))
   | Type_assert : forall (sigma:(map mident datatype)) (pi:(list (ident*
-      datatype)%type)) (p:fmla), (type_fmla sigma pi p) -> (type_stmt sigma
-      pi (Sassert p))
+      datatype)%type)) (p:fmla), (type_fmla sigma pi p) -> (type_expr sigma
+      pi (Eassert p) TYbool)
   | Type_while : forall (sigma:(map mident datatype)) (pi:(list (ident*
-      datatype)%type)) (guard:term) (body:stmt) (inv:fmla), (type_fmla sigma
-      pi inv) -> ((type_term sigma pi guard TYbool) -> ((type_stmt sigma pi
-      body) -> (type_stmt sigma pi (Swhile guard inv body)))).
+      datatype)%type)) (guard:expr) (body:expr) (inv:fmla) (ty:datatype),
+      (type_fmla sigma pi inv) -> ((type_expr sigma pi guard TYbool) ->
+      ((type_expr sigma pi body ty) -> (type_expr sigma pi (Ewhile guard inv
+      body) ty)))
+  | Type_Elet : forall (sigma:(map mident datatype)) (pi:(list (ident*
+      datatype)%type)) (x:ident) (e1:expr) (e2:expr) (ty1:datatype)
+      (ty2:datatype), (type_expr sigma pi e1 ty1) -> ((type_expr sigma
+      (Cons (x, ty1) pi) e2 ty2) -> (type_expr sigma pi (Elet x e1 e2) ty2)).
 
 (* Why3 assumption *)
 Definition env  := (map mident value).
@@ -323,32 +345,10 @@ Fixpoint eval_term(sigma:(map mident value)) (pi:(list (ident* value)%type))
       pi t2))
   end.
 
-(* Why3 assumption *)
-Inductive compatible : datatype -> value -> Prop :=
-  | Compatible_bool : forall (b:bool), (compatible TYbool (Vbool b))
-  | Compatible_int : forall (n:Z), (compatible TYint (Vint n))
-  | Compatible_void : (compatible TYunit Vvoid).
-
-(* Why3 assumption *)
-Definition existe_compatible(ty:datatype) (v:value): Prop :=
-  match ty with
-  | TYbool => exists b:bool, (v = (Vbool b))
-  | TYint => exists n:Z, (v = (Vint n))
-  | TYunit => (v = Vvoid)
-  end.
-
-(* Why3 assumption *)
-Definition compatible_env(sigma:(map mident value)) (sigmat:(map mident
-  datatype)) (pi:(list (ident* value)%type)) (pit:(list (ident*
-  datatype)%type)): Prop := (forall (id:mident), (compatible (get sigmat id)
-  (get sigma id))) /\ forall (id:ident), (compatible (get_vartype id pit)
-  (get_stack id pi)).
-
-Axiom eval_type_term : forall (t:term) (sigma:(map mident value)) (pi:(list
-  (ident* value)%type)) (sigmat:(map mident datatype)) (pit:(list (ident*
-  datatype)%type)) (ty:datatype), (compatible_env sigma sigmat pi pit) ->
-  ((type_term sigmat pit t ty) -> (existe_compatible ty (eval_term sigma pi
-  t))).
+Axiom eval_bool_term : forall (sigma:(map mident value)) (pi:(list (ident*
+  value)%type)) (sigmat:(map mident datatype)) (pit:(list (ident*
+  datatype)%type)) (t:term), (type_term sigmat pit t TYbool) ->
+  exists b:bool, ((eval_term sigma pi t) = (Vbool b)).
 
 (* Why3 assumption *)
 Fixpoint eval_fmla(sigma:(map mident value)) (pi:(list (ident* value)%type))
@@ -483,89 +483,133 @@ Definition valid_fmla(p:fmla): Prop := forall (sigma:(map mident value))
   (pi:(list (ident* value)%type)), (eval_fmla sigma pi p).
 
 (* Why3 assumption *)
-Fixpoint fresh_in_stmt(id:ident) (s:stmt) {struct s}: Prop :=
-  match s with
-  | Sskip => True
-  | (Sseq s1 s2) => (fresh_in_stmt id s1) /\ (fresh_in_stmt id s2)
-  | (Sassign _ t) => (fresh_in_term id t)
-  | (Sif t s1 s2) => (fresh_in_term id t) /\ ((fresh_in_stmt id s1) /\
-      (fresh_in_stmt id s2))
-  | (Sassert f) => (fresh_in_fmla id f)
-  | (Swhile cond inv body) => (fresh_in_term id cond) /\ ((fresh_in_fmla id
-      inv) /\ (fresh_in_stmt id body))
+Fixpoint fresh_in_expr(id:ident) (e:expr) {struct e}: Prop :=
+  match e with
+  | (Evalue _) => True
+  | (Ebin e1 op e2) => (fresh_in_expr id e1) /\ (fresh_in_expr id e2)
+  | (Evar v) => ~ (id = v)
+  | (Ederef _) => True
+  | (Eassign x e1) => (fresh_in_expr id e1)
+  | (Eseq e1 e2) => (fresh_in_expr id e1) /\ (fresh_in_expr id e2)
+  | (Elet v e1 e2) => (~ (id = v)) /\ ((fresh_in_expr id e1) /\
+      (fresh_in_expr id e2))
+  | (Eif e1 e2 e3) => (fresh_in_expr id e1) /\ ((fresh_in_expr id e2) /\
+      (fresh_in_expr id e3))
+  | (Eassert f) => (fresh_in_fmla id f)
+  | (Ewhile cond inv body) => (fresh_in_expr id cond) /\ ((fresh_in_fmla id
+      inv) /\ (fresh_in_expr id body))
   end.
 
 (* Why3 assumption *)
-Inductive one_step : (map mident value) -> (list (ident* value)%type) -> stmt
-  -> (map mident value) -> (list (ident* value)%type) -> stmt -> Prop :=
-  | one_step_assign : forall (sigma:(map mident value)) (sigma':(map mident
-      value)) (pi:(list (ident* value)%type)) (x:mident) (t:term),
-      (sigma' = (set sigma x (eval_term sigma pi t))) -> (one_step sigma pi
-      (Sassign x t) sigma' pi Sskip)
-  | one_step_seq_noskip : forall (sigma:(map mident value)) (sigma':(map
+Inductive one_step : (map mident value) -> (list (ident* value)%type) -> expr
+  -> (map mident value) -> (list (ident* value)%type) -> expr -> Prop :=
+  | one_step_var : forall (sigma:(map mident value)) (pi:(list (ident*
+      value)%type)) (v:ident), (one_step sigma pi (Evar v) sigma pi
+      (Evalue (get_stack v pi)))
+  | one_step_deref : forall (sigma:(map mident value)) (pi:(list (ident*
+      value)%type)) (v:mident), (one_step sigma pi (Ederef v) sigma pi
+      (Evalue (get sigma v)))
+  | one_step_bin_ctxt1 : forall (sigma:(map mident value)) (sigma':(map
       mident value)) (pi:(list (ident* value)%type)) (pi':(list (ident*
-      value)%type)) (s1:stmt) (s1':stmt) (s2:stmt), (one_step sigma pi s1
-      sigma' pi' s1') -> (one_step sigma pi (Sseq s1 s2) sigma' pi' (Sseq s1'
-      s2))
-  | one_step_seq_skip : forall (sigma:(map mident value)) (pi:(list (ident*
-      value)%type)) (s:stmt), (one_step sigma pi (Sseq Sskip s) sigma pi s)
+      value)%type)) (op:operator) (e1:expr) (e1':expr) (e2:expr),
+      (one_step sigma pi e1 sigma' pi' e1') -> (one_step sigma pi (Ebin e1 op
+      e2) sigma' pi' (Ebin e1' op e2))
+  | one_step_bin_ctxt2 : forall (sigma:(map mident value)) (sigma':(map
+      mident value)) (pi:(list (ident* value)%type)) (pi':(list (ident*
+      value)%type)) (op:operator) (v1:value) (e2:expr) (e2':expr),
+      (one_step sigma pi e2 sigma' pi' e2') -> (one_step sigma pi
+      (Ebin (Evalue v1) op e2) sigma' pi' (Ebin (Evalue v1) op e2'))
+  | one_step_bin_value : forall (sigma:(map mident value)) (pi:(list (ident*
+      value)%type)) (op:operator) (v1:value) (v2:value), (one_step sigma pi
+      (Ebin (Evalue v1) op (Evalue v2)) sigma pi (Evalue (eval_bin v1 op
+      v2)))
+  | one_step_assign_ctxt : forall (sigma:(map mident value)) (sigma':(map
+      mident value)) (pi:(list (ident* value)%type)) (pi':(list (ident*
+      value)%type)) (x:mident) (e:expr) (e':expr), (one_step sigma pi e
+      sigma' pi' e') -> (one_step sigma pi (Eassign x e) sigma' pi'
+      (Eassign x e'))
+  | one_step_assign_value : forall (sigma:(map mident value)) (sigma':(map
+      mident value)) (pi:(list (ident* value)%type)) (x:mident) (v:value),
+      (sigma' = (set sigma x v)) -> (one_step sigma pi (Eassign x (Evalue v))
+      sigma' pi (Evalue Vvoid))
+  | one_step_seq_ctxt : forall (sigma:(map mident value)) (sigma':(map mident
+      value)) (pi:(list (ident* value)%type)) (pi':(list (ident*
+      value)%type)) (e1:expr) (e1':expr) (e2:expr), (one_step sigma pi e1
+      sigma' pi' e1') -> (one_step sigma pi (Eseq e1 e2) sigma' pi' (Eseq e1'
+      e2))
+  | one_step_seq_value : forall (sigma:(map mident value)) (pi:(list (ident*
+      value)%type)) (e:expr), (one_step sigma pi (Eseq (Evalue Vvoid) e)
+      sigma pi e)
+  | one_step_let_ctxt : forall (sigma:(map mident value)) (sigma':(map mident
+      value)) (pi:(list (ident* value)%type)) (pi':(list (ident*
+      value)%type)) (id:ident) (e1:expr) (e1':expr) (e2:expr),
+      (one_step sigma pi e1 sigma' pi' e1') -> (one_step sigma pi (Elet id e1
+      e2) sigma' pi' (Elet id e1' e2))
+  | one_step_let_value : forall (sigma:(map mident value)) (pi:(list (ident*
+      value)%type)) (id:ident) (v:value) (e:expr), (one_step sigma pi
+      (Elet id (Evalue v) e) sigma (Cons (id, v) pi) e)
+  | one_step_if_ctxt : forall (sigma:(map mident value)) (sigma':(map mident
+      value)) (pi:(list (ident* value)%type)) (pi':(list (ident*
+      value)%type)) (e1:expr) (e1':expr) (e2:expr) (e3:expr), (one_step sigma
+      pi e1 sigma' pi' e1') -> (one_step sigma pi (Eif e1 e2 e3) sigma' pi'
+      (Eif e1' e2 e3))
   | one_step_if_true : forall (sigma:(map mident value)) (pi:(list (ident*
-      value)%type)) (t:term) (s1:stmt) (s2:stmt), ((eval_term sigma pi
-      t) = (Vbool true)) -> (one_step sigma pi (Sif t s1 s2) sigma pi s1)
+      value)%type)) (e1:expr) (e2:expr), (one_step sigma pi
+      (Eif (Evalue (Vbool true)) e1 e2) sigma pi e1)
   | one_step_if_false : forall (sigma:(map mident value)) (pi:(list (ident*
-      value)%type)) (t:term) (s1:stmt) (s2:stmt), ((eval_term sigma pi
-      t) = (Vbool false)) -> (one_step sigma pi (Sif t s1 s2) sigma pi s2)
+      value)%type)) (e1:expr) (e2:expr), (one_step sigma pi
+      (Eif (Evalue (Vbool false)) e1 e2) sigma pi e2)
   | one_step_assert : forall (sigma:(map mident value)) (pi:(list (ident*
       value)%type)) (f:fmla), (eval_fmla sigma pi f) -> (one_step sigma pi
-      (Sassert f) sigma pi Sskip)
+      (Eassert f) sigma pi (Evalue Vvoid))
   | one_step_while_true : forall (sigma:(map mident value)) (pi:(list (ident*
-      value)%type)) (cond:term) (inv:fmla) (body:stmt), (eval_fmla sigma pi
-      inv) -> (((eval_term sigma pi cond) = (Vbool true)) -> (one_step sigma
-      pi (Swhile cond inv body) sigma pi (Sseq body (Swhile cond inv body))))
+      value)%type)) (cond:expr) (body:expr) (inv:fmla), (eval_fmla sigma pi
+      inv) -> (one_step sigma pi (Ewhile (Evalue (Vbool true)) inv body)
+      sigma pi (Eseq body (Ewhile cond inv body)))
   | one_step_while_false : forall (sigma:(map mident value)) (pi:(list
-      (ident* value)%type)) (cond:term) (inv:fmla) (body:stmt),
-      (eval_fmla sigma pi inv) -> (((eval_term sigma pi
-      cond) = (Vbool false)) -> (one_step sigma pi (Swhile cond inv body)
-      sigma pi Sskip)).
+      (ident* value)%type)) (inv:fmla) (body:expr), (eval_fmla sigma pi
+      inv) -> (one_step sigma pi (Ewhile (Evalue (Vbool false)) inv body)
+      sigma pi (Evalue Vvoid)).
 
 (* Why3 assumption *)
 Inductive many_steps : (map mident value) -> (list (ident* value)%type)
-  -> stmt -> (map mident value) -> (list (ident* value)%type) -> stmt
+  -> expr -> (map mident value) -> (list (ident* value)%type) -> expr
   -> Z -> Prop :=
   | many_steps_refl : forall (sigma:(map mident value)) (pi:(list (ident*
-      value)%type)) (s:stmt), (many_steps sigma pi s sigma pi s 0%Z)
+      value)%type)) (s:expr), (many_steps sigma pi s sigma pi s 0%Z)
   | many_steps_trans : forall (sigma1:(map mident value)) (sigma2:(map mident
       value)) (sigma3:(map mident value)) (pi1:(list (ident* value)%type))
       (pi2:(list (ident* value)%type)) (pi3:(list (ident* value)%type))
-      (s1:stmt) (s2:stmt) (s3:stmt) (n:Z), (one_step sigma1 pi1 s1 sigma2 pi2
-      s2) -> ((many_steps sigma2 pi2 s2 sigma3 pi3 s3 n) ->
-      (many_steps sigma1 pi1 s1 sigma3 pi3 s3 (n + 1%Z)%Z)).
+      (s1:expr) (s2:expr) (s3:expr) (n:Z), (0%Z < n)%Z -> ((one_step sigma1
+      pi1 s1 sigma2 pi2 s2) -> ((many_steps sigma2 pi2 s2 sigma3 pi3 s3
+      (n - 1%Z)%Z) -> (many_steps sigma1 pi1 s1 sigma3 pi3 s3 n))).
 
 Axiom steps_non_neg : forall (sigma1:(map mident value)) (sigma2:(map mident
   value)) (pi1:(list (ident* value)%type)) (pi2:(list (ident* value)%type))
-  (s1:stmt) (s2:stmt) (n:Z), (many_steps sigma1 pi1 s1 sigma2 pi2 s2 n) ->
+  (s1:expr) (s2:expr) (n:Z), (many_steps sigma1 pi1 s1 sigma2 pi2 s2 n) ->
   (0%Z <= n)%Z.
 
 Axiom many_steps_seq : forall (sigma1:(map mident value)) (sigma3:(map mident
   value)) (pi1:(list (ident* value)%type)) (pi3:(list (ident* value)%type))
-  (s1:stmt) (s2:stmt) (n:Z), (many_steps sigma1 pi1 (Sseq s1 s2) sigma3 pi3
-  Sskip n) -> exists sigma2:(map mident value), exists pi2:(list (ident*
-  value)%type), exists n1:Z, exists n2:Z, (many_steps sigma1 pi1 s1 sigma2
-  pi2 Sskip n1) /\ ((many_steps sigma2 pi2 s2 sigma3 pi3 Sskip n2) /\
-  (n = ((1%Z + n1)%Z + n2)%Z)).
+  (e1:expr) (e2:expr) (n:Z), (many_steps sigma1 pi1 (Eseq e1 e2) sigma3 pi3
+  (Evalue Vvoid) n) -> exists sigma2:(map mident value), exists pi2:(list
+  (ident* value)%type), exists n1:Z, exists n2:Z, (many_steps sigma1 pi1 e1
+  sigma2 pi2 (Evalue Vvoid) n1) /\ ((many_steps sigma2 pi2 e2 sigma3 pi3
+  (Evalue Vvoid) n2) /\ (n = ((1%Z + n1)%Z + n2)%Z)).
 
 (* Why3 assumption *)
-Definition valid_triple(p:fmla) (s:stmt) (q:fmla): Prop := forall (sigma:(map
+Definition valid_triple(p:fmla) (e:expr) (q:fmla): Prop := forall (sigma:(map
   mident value)) (pi:(list (ident* value)%type)), (eval_fmla sigma pi p) ->
   forall (sigma':(map mident value)) (pi':(list (ident* value)%type)) (n:Z),
-  (many_steps sigma pi s sigma' pi' Sskip n) -> (eval_fmla sigma' pi' q).
+  (many_steps sigma pi e sigma' pi' (Evalue Vvoid) n) -> (eval_fmla sigma'
+  pi' q).
 
 (* Why3 assumption *)
-Definition total_valid_triple(p:fmla) (s:stmt) (q:fmla): Prop :=
+Definition total_valid_triple(p:fmla) (e:expr) (q:fmla): Prop :=
   forall (sigma:(map mident value)) (pi:(list (ident* value)%type)),
   (eval_fmla sigma pi p) -> exists sigma':(map mident value),
-  exists pi':(list (ident* value)%type), exists n:Z, (many_steps sigma pi s
-  sigma' pi' Sskip n) /\ (eval_fmla sigma' pi' q).
+  exists pi':(list (ident* value)%type), exists n:Z, (many_steps sigma pi e
+  sigma' pi' (Evalue Vvoid) n) /\ (eval_fmla sigma' pi' q).
 
 Axiom set1 : forall (a:Type) {a_WT:WhyType a}, Type.
 Parameter set1_WhyType : forall (a:Type) {a_WT:WhyType a}, WhyType (set1 a).
@@ -666,87 +710,92 @@ Axiom assigns_union_right : forall (sigma:(map mident value)) (sigma':(map
   sigma') -> (assigns sigma (union s1 s2) sigma').
 
 (* Why3 assumption *)
-Fixpoint stmt_writes(s:stmt) (w:(set1 mident)) {struct s}: Prop :=
+Fixpoint expr_writes(s:expr) (w:(set1 mident)) {struct s}: Prop :=
   match s with
-  | (Sskip|(Sassert _)) => True
-  | (Sassign id _) => (mem1 id w)
-  | (Sseq s1 s2) => (stmt_writes s1 w) /\ (stmt_writes s2 w)
-  | (Sif t s1 s2) => (stmt_writes s1 w) /\ (stmt_writes s2 w)
-  | (Swhile _ _ body) => (stmt_writes body w)
+  | ((Evalue _)|((Evar _)|((Ederef _)|(Eassert _)))) => True
+  | (Eassign id _) => (mem1 id w)
+  | (Eseq e1 e2) => (expr_writes e1 w) /\ (expr_writes e2 w)
+  | (Eif e1 e2 e3) => (expr_writes e1 w) /\ ((expr_writes e2 w) /\
+      (expr_writes e3 w))
+  | (Ewhile cond _ body) => (expr_writes cond w) /\ (expr_writes body w)
+  | (Ebin e1 o e2) => (expr_writes e1 w) /\ (expr_writes e2 w)
+  | (Elet id e1 e2) => (expr_writes e1 w) /\ (expr_writes e2 w)
   end.
 
-Parameter fresh_from: fmla -> stmt -> ident.
+Parameter fresh_from: fmla -> expr -> ident.
 
-Axiom fresh_from_fmla : forall (s:stmt) (f:fmla),
+Axiom fresh_from_fmla : forall (s:expr) (f:fmla),
   (fresh_in_fmla (fresh_from f s) f).
 
-Axiom fresh_from_stmt : forall (s:stmt) (f:fmla),
-  (fresh_in_stmt (fresh_from f s) s).
+Axiom fresh_from_expr : forall (s:expr) (f:fmla),
+  (fresh_in_expr (fresh_from f s) s).
 
-Parameter abstract_effects: stmt -> fmla -> fmla.
+Parameter abstract_effects: expr -> fmla -> fmla.
 
 Axiom abstract_effects_generalize : forall (sigma:(map mident value))
-  (pi:(list (ident* value)%type)) (s:stmt) (f:fmla), (eval_fmla sigma pi
+  (pi:(list (ident* value)%type)) (s:expr) (f:fmla), (eval_fmla sigma pi
   (abstract_effects s f)) -> (eval_fmla sigma pi f).
 
-Axiom abstract_effects_monotonic : forall (s:stmt) (f:fmla),
+Axiom abstract_effects_monotonic : forall (s:expr) (f:fmla),
   forall (sigma:(map mident value)) (pi:(list (ident* value)%type)),
   (eval_fmla sigma pi f) -> forall (sigma1:(map mident value)) (pi1:(list
   (ident* value)%type)), (eval_fmla sigma1 pi1 (abstract_effects s f)).
 
 (* Why3 assumption *)
-Fixpoint wp(s:stmt) (q:fmla) {struct s}: fmla :=
-  match s with
-  | Sskip => q
-  | (Sassert f) => (Fand f (Fimplies f q))
-  | (Sseq s1 s2) => (wp s1 (wp s2 q))
-  | (Sassign x t) => let id := (fresh_from q s) in (Flet id t (msubst q x
-      id))
-  | (Sif t s1 s2) => (Fand (Fimplies (Fterm t) (wp s1 q))
-      (Fimplies (Fnot (Fterm t)) (wp s2 q)))
-  | (Swhile cond inv body) => (Fand inv (abstract_effects body
-      (Fand (Fimplies (Fand (Fterm cond) inv) (wp body inv))
-      (Fimplies (Fand (Fnot (Fterm cond)) inv) q))))
+Fixpoint wp(e:expr) (q:fmla) {struct e}: fmla :=
+  match e with
+  | (Evalue v) => (Flet result (Tvalue v) q)
+  | (Evar v) => (Flet result (Tvar v) q)
+  | (Ederef v) => (Flet result (Tderef v) q)
+  | (Eassert f) => (Fand f (Fimplies f q))
+  | (Eseq e1 e2) => (wp e1 (wp e2 q))
+  | (Elet id e1 e2) => (wp e1 (Flet id (Tvar result) (wp e2 q)))
+  | (Ebin e1 op e2) => let t1 := (fresh_from q e) in let t2 :=
+      (fresh_from (Fand (Fterm (Tvar t1)) q) e) in let q' := (Flet result
+      (Tbin (Tvar t1) op (Tvar t2)) q) in let f := (wp e2 (Flet t2
+      (Tvar result) q')) in (wp e1 (Flet t1 (Tvar result) f))
+  | (Eassign x e1) => let id := (fresh_from q e1) in let q' := (Flet result
+      (Tvalue Vvoid) q) in (wp e1 (Flet id (Tvar result) (msubst q' x id)))
+  | (Eif e1 e2 e3) => let f := (Fand (Fimplies (Fterm (Tvar result)) (wp e2
+      q)) (Fimplies (Fnot (Fterm (Tvar result))) (wp e3 q))) in (wp e1 f)
+  | (Ewhile cond inv body) => (Fand inv (abstract_effects body (wp cond
+      (Fand (Fimplies (Fand (Fterm (Tvar result)) inv) (wp body inv))
+      (Fimplies (Fand (Fnot (Fterm (Tvar result))) inv) q)))))
   end.
 
 Axiom abstract_effects_writes : forall (sigma:(map mident value)) (pi:(list
-  (ident* value)%type)) (s:stmt) (q:fmla), (eval_fmla sigma pi
+  (ident* value)%type)) (s:expr) (q:fmla), (eval_fmla sigma pi
   (abstract_effects s q)) -> (eval_fmla sigma pi (wp s (abstract_effects s
   q))).
 
-Axiom monotonicity : forall (s:stmt) (p:fmla) (q:fmla),
+Axiom monotonicity : forall (s:expr) (p:fmla) (q:fmla),
   (valid_fmla (Fimplies p q)) -> (valid_fmla (Fimplies (wp s p) (wp s q))).
 
-Axiom distrib_conj : forall (s:stmt) (sigma:(map mident value)) (pi:(list
+Axiom distrib_conj : forall (s:expr) (sigma:(map mident value)) (pi:(list
   (ident* value)%type)) (p:fmla) (q:fmla), ((eval_fmla sigma pi (wp s p)) /\
   (eval_fmla sigma pi (wp s q))) -> (eval_fmla sigma pi (wp s (Fand p q))).
 
-Axiom wp_reduction : forall (sigma:(map mident value)) (sigma':(map mident
-  value)) (pi:(list (ident* value)%type)) (pi':(list (ident* value)%type))
-  (s:stmt) (s':stmt), (one_step sigma pi s sigma' pi' s') -> forall (q:fmla),
-  (eval_fmla sigma pi (wp s q)) -> (eval_fmla sigma' pi' (wp s' q)).
-
 (* Why3 goal *)
-Theorem progress : forall (s:stmt),
+Theorem wp_reduction : forall (sigma:(map mident value)) (sigma':(map mident
+  value)) (pi:(list (ident* value)%type)) (pi':(list (ident* value)%type))
+  (s:expr),
   match s with
-  | Sskip => True
-  | (Sassign m t) => True
-  | (Sseq s1 s2) => True
-  | (Sif t s1 s2) => True
-  | (Sassert f) => forall (sigma:(map mident value)) (pi:(list (ident*
-      value)%type)) (sigmat:(map mident datatype)) (pit:(list (ident*
-      datatype)%type)) (q:fmla), (compatible_env sigma sigmat pi pit) ->
-      ((type_stmt sigmat pit s) -> ((eval_fmla sigma pi (wp s q)) ->
-      ((~ (s = Sskip)) -> exists sigma':(map mident value), exists pi':(list
-      (ident* value)%type), exists s':stmt, (one_step sigma pi s sigma' pi'
-      s'))))
-  | (Swhile t f s1) => True
+  | (Evalue v) => True
+  | (Ebin e o e1) => True
+  | (Evar i) => forall (s':expr), (one_step sigma pi s sigma' pi' s') ->
+      forall (q:fmla), (eval_fmla sigma pi (wp s q)) -> (eval_fmla sigma' pi'
+      (wp s' q))
+  | (Ederef m) => True
+  | (Eassign m e) => True
+  | (Eseq e e1) => True
+  | (Elet i e e1) => True
+  | (Eif e e1 e2) => True
+  | (Eassert f) => True
+  | (Ewhile e f e1) => True
   end.
 destruct s; auto.
-simpl.
-intros sigma pi sigmat pit q H H1 (H2 & H3) H4.
-do 3 eexists.
-apply one_step_assert; auto.
+intros e' H q H1.
+inversion H; subst; auto.
 Qed.
 
 
